Restructure code and improve automation

src/Env.v
@@ -1,6 +1,7 @@
 From MCore Require Import Syntax Tactics.
-From TLC Require Import LibList.
-Import LibListNotation.
+From TLC Require Import LibNat LibList.
+
+Open Scope nat_scope.
 
 Module Env (P : PAT).
   Module S := Syntax P.
@@ -17,11 +18,11 @@ Module Env (P : PAT).
   | BindTvar  : kind -> binding
   | BindVar   : type -> binding
   | BindMatch : match_assum -> binding
-  | SkipTvar  : binding
-  | SkipVar   : binding
   .
 
   Definition env : Type := list binding.
+
+  Definition empty_env : env := nil.
 
   Definition is_tname (b : binding) : Prop := match b with BindTname => True | _ => False end.
   Definition tnames   (Gamma : env) : env := filter is_tname Gamma.
@@ -29,35 +30,28 @@ Module Env (P : PAT).
   Definition is_con (b : binding) : Prop := match b with BindCon _ _ _ => True | _ => False end.
   Definition cons   (Gamma : env) : env := filter is_con Gamma.
 
-  Definition is_tvar (b : binding) : Prop :=
-    match b with BindTvar _ => True | SkipTvar => True | _ => False end.
-  #[export]
-  Hint Unfold is_tvar : mcore.
+  Definition is_tvar (b : binding) : Prop := match b with BindTvar _ => True | _ => False end.
   Definition tvars   (Gamma : env) : env := filter is_tvar Gamma.
 
-  Definition is_var (b : binding) : Prop :=
-    match b with BindVar _ => True | SkipVar => True | _ => False end.
-  #[export]
-  Hint Unfold is_var : mcore.
+  Definition is_var (b : binding) : Prop := match b with BindVar _ => True | _ => False end.
   Definition vars   (Gamma : env) : env := filter is_var Gamma.
-
 
   Definition is_match (b : binding) : Prop := match b with BindMatch _ => True | _ => False end.
   Definition matches  (Gamma : env) : env := filter is_match Gamma.
 
+  Definition binds (n : nat) (b : binding) (Gamma : env) : Prop := Nth n Gamma b.
+
   Definition tname_in (T : tname) (Gamma : env) : Prop :=
-    Nth T Gamma BindTname.
+    binds T BindTname (tnames Gamma).
 
   Definition con_in (K : con) (d : data) (ty : type) (T : tname) (Gamma : env) : Prop :=
-    Nth K Gamma (BindCon d ty T).
+    binds K (BindCon d ty T) (cons Gamma).
 
   Definition tvar_in (tv : tvar) (k : kind) (Gamma : env) : Prop :=
-    Nth tv Gamma (BindTvar k).
+    binds tv (BindTvar k) (tvars Gamma).
 
   Definition var_in (v : var) (ty : type) (Gamma : env) : Prop :=
-    Nth v Gamma (BindVar ty).
-
-  Definition empty_env : env := [ ].
+    binds v (BindVar ty) (vars Gamma).
 
 
   Create HintDb rew_env.
@@ -89,12 +83,27 @@ Module Env (P : PAT).
       vars (b :: Gamma) =
         match b with
         | BindVar _ => b :: vars Gamma
-        | SkipVar   => b :: vars Gamma
         | _         => vars Gamma
         end.
   Proof. intros ; destruct b ; unfolds ; unfolds is_var ; rew_listx ; case_if*. Qed.
 
   #[export]
   Hint Rewrite vars_app vars_cons : rew_env.
+
+  Lemma binds_app_middle_inv :
+    forall x y1 y2 G1 G2,
+      binds x y1 (G1 ++ y2 :: G2) ->
+      x < length G1 /\ binds x y1 (G1 ++ G2)
+      \/ x = length G1 /\ y1 = y2
+      \/ x > length G1 /\ binds (x - 1) y1 (G1 ++ G2).
+  Proof.
+    introv Hvar.
+    lets [ in_G1 | (m' & Heqm' & in_G2') ] : Nth_app_inv Hvar.
+    { left. lets Hlt : Nth_inbound in_G1. nat_comp_to_peano.
+      split*. apply* Nth_app_l. }
+    { right. lets [ (Heq0 & Heqty) | (m & Heqm & in_G2) ] : Nth_cons_inv in_G2' ; subst.
+      { left*. }
+      { right. split*. simple_math. applys_eq (>> Nth_app_r G1 in_G2). nat_math. } }
+  Qed.
 
 End Env.
